added vars

VarLang1.v
@@ -14,8 +14,15 @@ Set Implicit Arguments.
 
 Inductive binop : Set := Plus | Times.
 
+Definition var := nat.
+Definition vars := var -> nat.
+Definition set (vs : vars) (v : var) (n : nat) : vars :=
+  fun v' => if beq_nat v v' then n else vs v'.
+Definition vs0 := fun v: var => 0.
+
 Inductive exp : Set :=
 | Const : nat -> exp
+| Var : var -> exp
 | Binop : binop -> exp -> exp -> exp.
 
 Definition binopDenote (b : binop) : nat -> nat -> nat :=
@@ -24,14 +31,26 @@ Definition binopDenote (b : binop) : nat -> nat -> nat :=
     | Times => mult
   end.
 
-Fixpoint expDenote (e : exp) : nat :=
+Fixpoint expDenote (vs : vars) (e : exp) : nat :=
   match e with
     | Const n => n
-    | Binop b e1 e2 => (binopDenote b) (expDenote e1) (expDenote e2)
+    | Var v => vs v
+    | Binop b e1 e2 => (binopDenote b) (expDenote vs e1) (expDenote vs e2)
   end.
 
-Eval simpl in expDenote (Const 42).
+Example test_const:
+  expDenote vs0 (Const 42) = 42.
+Proof. simpl. reflexivity. Qed.
 
-Eval simpl in expDenote (Binop Plus (Const 2) (Const 2)).
+Example test_plus:
+  expDenote vs0 (Binop Plus (Const 2) (Const 2)) = 4.
+Proof. simpl. reflexivity. Qed.
 
-Eval simpl in expDenote (Binop Times (Binop Plus (Const 2) (Const 2)) (Const 7)).
+Example test_times:
+  expDenote vs0 (Binop Times (Binop Plus (Const 2) (Const 2)) (Const 7)) = 28.
+Proof. simpl. reflexivity. Qed.
+
+Example test_var:
+  expDenote (set vs0 0 1) (Binop Plus (Var 0) (Var 0)) = 2.
+Proof. auto. Qed.
+
